tests/e2e/fib_iter.js
@@ -1,0 +1,16 @@
+// Iterative Fibonacci (ECMA-262 §13.7.4)
+function fib(n) {
+  var a = 0;
+  var b = 1;
+  var i = 0;
+  while (i < n) {
+    var temp = b;
+    b = a + b;
+    a = temp;
+    i = i + 1;
+  }
+  return a;
+}
+console.log(fib(0));
+console.log(fib(1));
+console.log(fib(10));
