tests/e2e/nested_obj_method.js
@@ -1,0 +1,4 @@
+// Test nested object property access and method-like calls
+var obj = { x: 10, y: 20 };
+var sum = obj.x + obj.y;
+console.log(sum);
