tests/e2e/obj_bracket.js
@@ -1,0 +1,4 @@
+// Test object bracket notation (ECMA-262 §12.3.2)
+var obj = { a: 1, b: 2, c: 3 };
+var key = "b";
+console.log(obj[key]);
